examples/TestEx.thy
@@ -5,6 +5,7 @@ begin
 definition "x == True"
 
 lemma test2: x
+unfolding x_def
       by auto (* FAILS *)
 
 
