isabelle-thys/Basic_Rules.thy
@@ -1,0 +1,164 @@
+theory Basic_Rules
+  imports Relational_Hoare
+begin
+
+lemma skip_rule:
+  shows "qrhl B [] [] B"
+  by (cheat skip_rule)
+
+lemma conseq_rule:
+  assumes "A \<le> A'" and "B' \<le> B"
+  assumes "qrhl A' b c B'"
+  shows "qrhl A b c B"
+  by (cheat conseq_rule)
+
+lemma sym_rule:
+  assumes "qrhl (index_flip_expression A) c b (index_flip_expression B)"
+  shows "qrhl A b c B"
+  by (cheat sym_rule)
+
+lemma assign1_rule:
+  fixes A B x e
+  defines "x1 == index_var True x"
+  defines "e1 == index_expression True e"
+  defines "A == subst_expression [substitute1 x1 e1] B"
+  shows "qrhl A [assign x e] [] B"
+  by (cheat assign1_rule)
+
+(* TODO move *)
+lemma index_flip_subst_expression: "index_flip_expression (subst_expression \<sigma> e) 
+  = subst_expression (map index_flip_substitute1 \<sigma>) (index_flip_expression e)"
+  by (cheat index_flip_subst_expression)
+
+(* TODO move *)
+lemma index_flip_var_index_var_raw[simp]: "index_flip_var_raw (index_var_raw left x) = index_var_raw (\<not> left) x"
+  apply transfer
+  by (auto simp: index_flip_name_def)
+
+(* TODO move *)
+lemma index_flip_var_index_var[simp]: "index_flip_var (index_var left x) = index_var (\<not>left) x"
+  apply transfer by simp
+
+(* TODO move *)
+lemma index_flip_expression_index_expression: "index_flip_expression (index_expression left x) =
+  index_expression (\<not>left) x"
+  apply transfer apply auto
+  using image_iff by fastforce
+
+lemma expression_vars_index_flip_expression: "expression_vars (index_flip_expression e) = index_flip_var_raw ` expression_vars e"
+  by (simp add: expression_vars.rep_eq index_flip_expression.rep_eq split_beta)
+
+lemma expression_eval_index_flip_expression: "expression_eval (index_flip_expression e) = 
+  expression_eval e o index_flip_mem2"
+  unfolding o_def
+  by (simp add: expression_eval.rep_eq index_flip_expression.rep_eq split_beta)
+
+
+lemma expression_eqI: "expression_vars e = expression_vars f \<Longrightarrow> expression_eval e = expression_eval f \<Longrightarrow> e = f"
+  apply transfer by auto
+
+(* TODO move *)
+lemma index_flip_expression_map_expression': "index_flip_expression (map_expression' f ez)
+  = map_expression' f (index_flip_expression o ez)"
+proof (cases "\<forall>z. expression_vars (ez z) = expression_vars (ez undefined)")
+  case True
+  then have True': "expression_vars (index_flip_expression (ez z)) = expression_vars (index_flip_expression (ez undefined))" for z
+    apply transfer
+    apply simp
+    by (metis (mono_tags, lifting) fst_conv split_beta)
+
+  from True have "expression_vars (map_expression' f ez) = expression_vars (ez undefined)"
+    apply transfer by (simp add: fst_def)
+  hence "expression_vars (index_flip_expression (map_expression' f ez)) 
+       = index_flip_var_raw ` expression_vars (ez undefined)"
+    unfolding expression_vars_index_flip_expression by simp
+  moreover from True' have "expression_vars (map_expression' f (index_flip_expression o ez)) 
+      = expression_vars (index_flip_expression (ez undefined))"
+    unfolding o_def apply transfer by (auto simp: fst_def)
+  moreover have "expression_vars (index_flip_expression (ez undefined))
+      = index_flip_var_raw ` expression_vars (ez undefined)"
+    unfolding expression_vars_index_flip_expression by simp
+  ultimately have vars: "expression_vars (index_flip_expression (map_expression' f ez))
+                 = expression_vars (map_expression' f (index_flip_expression o ez))"
+    by simp
+
+  from True have "expression_eval (map_expression' f ez) = (\<lambda>m. f (\<lambda>z. expression_eval (ez z) m))"
+    apply transfer by (auto simp: fst_def snd_def)
+  hence "expression_eval (index_flip_expression (map_expression' f ez)) 
+       = (\<lambda>m. f (\<lambda>z. expression_eval (ez z) (index_flip_mem2 m)))"
+    unfolding expression_eval_index_flip_expression by (simp add: o_def)
+  moreover from True' have "expression_eval (map_expression' f (index_flip_expression o ez)) 
+      = (\<lambda>m. f (\<lambda>z. expression_eval (index_flip_expression (ez z)) m))"
+    unfolding o_def apply transfer by (auto simp: fst_def snd_def)
+  moreover have "expression_eval (ez z) (index_flip_mem2 m) = expression_eval (index_flip_expression (ez z)) m" for m z
+    apply transfer by (simp add: split_beta)
+  ultimately have eval: "expression_eval (index_flip_expression (map_expression' f ez))
+                 = expression_eval (map_expression' f (index_flip_expression o ez))"
+    by simp
+  
+  from vars eval show ?thesis
+    by (rule expression_eqI)
+next
+  case False
+  then have False': "\<not> (\<forall>z. expression_vars (index_flip_expression (ez z)) = expression_vars (index_flip_expression (ez undefined)))"
+    apply transfer
+    apply (simp add: case_prod_beta)
+    using index_flip_var_raw_inject by blast
+
+  have "map_expression' f ez = const_expression undefined"
+    apply (subst Rep_expression_inject[symmetric])
+    using False by (auto simp: map_expression'.rep_eq expression_vars.rep_eq case_prod_beta)
+  then have "index_flip_expression (map_expression' f ez) = const_expression undefined"
+    by simp
+  also from False' have "map_expression' f (index_flip_expression o ez) = const_expression undefined"
+    apply (subst Rep_expression_inject[symmetric])
+    using False by (auto simp: map_expression'.rep_eq expression_vars.rep_eq case_prod_beta)
+  finally show ?thesis by metis
+qed
+
+
+(* TODO move *)
+lemma index_flip_expression_pair_expression: "index_flip_expression (pair_expression e1 e2)
+  = pair_expression (index_flip_expression e1) (index_flip_expression e2)"
+  apply transfer by auto
+
+(* TODO move *)
+lemma index_flip_map_expression2': "index_flip_expression (map_expression2' f e1 e2) = 
+  map_expression2' f (index_flip_expression e1) (index_flip_expression o e2)"
+  unfolding map_expression2'_def by (simp add: index_flip_expression_pair_expression index_flip_expression_map_expression' o_def)
+
+lemma assign2_rule:
+  fixes A B x e
+  defines "x1 == index_var False x"
+  defines "e1 == index_expression False e"
+  defines "A == subst_expression [substitute1 x1 e1] B"
+  shows "qrhl A [] [assign x e] B"
+  using [[simproc del: index_var]]
+  apply (rule sym_rule)
+  apply (simp add: assms index_flip_subst_expression index_flip_substitute1 index_flip_var_index_var index_flip_expression_index_expression)
+  by (rule assign1_rule)
+
+lemma sample1_rule:
+  fixes A B x e
+  defines "x1 == index_var True x"
+  defines "e1 == index_expression True e"
+  defines "\<And>z. B' z == subst_expression [substitute1 x1 (const_expression z)] B"
+  defines "A == map_expression2' (\<lambda>e1 B'. Cla[weight e1 = 1] \<sqinter> (INF z:supp e1. B' z)) e1 B'"
+  shows "qrhl A [sample x e] [] B"
+  by (cheat sample1_rule)
+
+lemma sample2_rule:
+  fixes A B x e
+  defines "x1 == index_var False x"
+  defines "e1 == index_expression False e"
+  defines "\<And>z. B' z == subst_expression [substitute1 x1 (const_expression z)] B"
+  defines "A == map_expression2' (\<lambda>e1 B'. Cla[weight e1 = 1] \<sqinter> (INF z:supp e1. B' z)) e1 B'"
+  shows "qrhl A [] [sample x e] B"
+  using [[simproc del: index_var]]
+  apply (rule sym_rule)
+  apply (simp add: assms index_flip_subst_expression index_flip_substitute1 
+      index_flip_var_index_var index_flip_expression_index_expression
+      index_flip_map_expression2' o_def)
+  by (rule sample1_rule)
+
+end
