isabelle-thys/Weakest_Precondition.thy
@@ -1,48 +1,6 @@
 theory Weakest_Precondition
-  imports Tactics
+  imports Tactics Basic_Rules
 begin
-
-lemma skip_rule:
-  shows "qrhl B [] [] B"
-  by (cheat skip_rule)
-
-(* TODO define sym_rule *)
-
-lemma assign1_rule:
-  fixes A B x e
-  defines "x1 == index_var True x"
-  defines "e1 == index_expression True e"
-  defines "A == subst_expression [substitute1 x1 e1] B"
-  shows "qrhl A [assign x e] [] B"
-  by (cheat assign1_rule)
-
-lemma assign2_rule:
-  fixes A B x e
-  defines "x1 == index_var False x"
-  defines "e1 == index_expression False e"
-  defines "A == subst_expression [substitute1 x1 e1] B"
-  shows "qrhl A [] [assign x e] B"
-(* TODO: derive from assign1_rule by sym_rule *)
-  by (cheat assign2_rule)
-
-lemma sample1_rule:
-  fixes A B x e
-  defines "x1 == index_var True x"
-  defines "e1 == index_expression True e"
-  defines "\<And>z. B' z == subst_expression [substitute1 x1 (const_expression z)] B"
-  defines "A == map_expression2' (\<lambda>e1 B'. Cla[weight e1 = 1] \<sqinter> (INF z:supp e1. B' z)) e1 B'"
-  shows "qrhl A [sample x e] [] B"
-  by (cheat sample1_rule)
-
-lemma sample2_rule:
-  fixes A B x e
-  defines "x1 == index_var False x"
-  defines "e1 == index_expression False e"
-  defines "\<And>z. B' z == subst_expression [substitute1 x1 (const_expression z)] B"
-  defines "A == map_expression2' (\<lambda>e1 B'. Cla[weight e1 = 1] \<sqinter> (INF z:supp e1. B' z)) e1 B'"
-  shows "qrhl A [] [sample x e] B"
-(* TODO: derive from assign1_rule by sym_rule *)
-  by (cheat sample2_rule)
 
 lemma wp1_assign_tac:
   fixes A B x e
